Foundation/Modal/Neighborhood/Completeness.lean
@@ -1,0 +1,5 @@
+import Foundation.Modal.MaximalConsistentSet
+
+namespace LO.Modal
+
+end LO.Modal
